compiler/kernel-template/coq/Extract.v
@@ -3,9 +3,11 @@ Require Import KrakenBase.
 Require Import Kernel.
 
 Extract Constant KrakenBase.chan => "KrakenBaseImpl.chan".
+Extract Constant KrakenBase.chan_eq => "KrakenBaseImpl.chan_eq".
 Extract Constant KrakenBase.fdesc => "KrakenBaseImpl.fdesc".
 Extract Constant KrakenBase.exec => "KrakenBaseImpl.exec".
 Extract Constant KrakenBase.call => "KrakenBaseImpl.call".
+Extract Constant KrakenBase.select => "KrakenBaseImpl.select".
 Extract Constant KrakenBase.recv => "KrakenBaseImpl.recv".
 Extract Constant KrakenBase.send => "KrakenBaseImpl.send".
 Extract Constant KrakenBase.recv_fd => "KrakenBaseImpl.recv_fd".
